Pop.lean
@@ -2,3 +2,4 @@ import Pop.States
 import Pop.Test
 import Pop.Pop
 import Pop.Program
+import Pop.Exploration
