Pop/Exploration.lean
@@ -1,0 +1,227 @@
+import Pop.States
+import Lean
+import Pop.Pop
+import Pop.Util
+import Std.Data
+open Std.HashMap
+open Util
+
+namespace Pop
+
+variable {ArchReqType : Type 0} [BEq ArchReqType] [Inhabited ArchReqType]
+
+abbrev ProgramState := Array (Array (@Transition ArchReqType))
+
+def ProgramState.getAvailable (prog : @ProgramState ArchReqType) : List (@Transition ArchReqType) := Id.run do
+  let mut res := []
+  for thread in prog do
+    if h : thread.size > 0 then
+    res := thread[thread.size - 1]'(by apply n_minus_one_le_n h) :: res
+  return res
+
+def ProgramState.removeTransition (prog : @ProgramState ArchReqType) (transition : (@Transition ArchReqType))
+  : @ProgramState ArchReqType := Id.run do
+  let mut res := #[]
+  let mut thread' := #[]
+  for thread in prog do
+    thread' := thread.erase transition
+    res := res.push thread'
+  return res
+
+def Request.possiblePropagateTransitions (req : @Request ArchReqType) (state :  @SystemState ArchReqType) : List (@Transition ArchReqType) :=
+  let threads := state.system.threads.removeAll req.propagated_to
+  --dbg_trace s!"Req {req.id} has not propagated to {threads}"
+  let threads_valid := threads.filter (state.canPropagate req.id)
+  --dbg_trace s!"Req {req.id} can propagate to {threads_valid}"
+  threads_valid.map λ th => Transition.propagateToThread req.id th
+
+def SystemState.possiblePropagateTransitions (state :  @SystemState ArchReqType) : List (@Transition ArchReqType) :=
+  let requests := filterNones state.requests.val.toList
+  let requests_not_fully_propagated := requests.filter λ r => ! (@Request.fullyPropagated ArchReqType state.system.scopes r state.system.scopes.systemScope)
+  let removedIds := state.removed.map Request.id
+  let requests_active := requests_not_fully_propagated.filter λ r => (state.seen.elem r.id) && (!removedIds.elem r.id)
+  -- dbg_trace s!"active requests: {requests_active}"
+  List.join $ requests_active.map λ r => r.possiblePropagateTransitions state
+
+def Request.possibleSatisfyTransitions (read : @Request ArchReqType) (state : @SystemState ArchReqType) : List (@Transition ArchReqType) :=
+  if !read.isRead then [] else
+    let requests := filterNones state.requests.val.toList
+    let writes_propagated_eq := requests.filter λ write => write.isWrite && write.propagated_to == read.propagated_to
+    --dbg_trace s!"writes with eq propagation to {read.id}: {writes_propagated_eq}"
+    let write_ids := writes_propagated_eq.map Request.id
+    let writes_valid := write_ids.filter (λ write => state.canSatisfyRead read.id write) -- should be length 1
+    --dbg_trace s!"valid writes for transition: {writes_valid}"
+    writes_valid.map $ Transition.satisfyRead read.id
+
+def SystemState.possibleSatisfyTransitions (state :  @SystemState ArchReqType) : List (@Transition ArchReqType) :=
+  let requests := filterNones state.requests.val.toList
+  let unsatisfied_reads := requests.filter λ r => r.isRead && !(state.isSatisfied r.id)
+  List.join $ unsatisfied_reads.map λ r => r.possibleSatisfyTransitions state
+
+def SystemState.possibleTransitions (state : @SystemState ArchReqType) (unaccepted : ProgramState) :=
+  let allaccepts := unaccepted.map λ th => th.filter Transition.isAccept
+  let accepts := ProgramState.getAvailable allaccepts
+  accepts ++ state.possibleSatisfyTransitions ++ state.possiblePropagateTransitions
+
+def SystemState.hasUnsatisfiedReads (state : @SystemState ArchReqType) :=
+  let requests := filterNones state.requests.val.toList
+  let reads := requests.filter Request.isRead
+  let readids := reads.map Request.id
+  let unsatisfied := readids.filter state.isSatisfied
+  unsatisfied != []
+
+def SystemState.isDeadlocked (state : SystemState) (unaccepted : @ProgramState ArchReqType) :=
+  let transitions := state.possibleTransitions unaccepted
+  transitions == [] && state.hasUnsatisfiedReads
+
+-- This should be a monad transformer or smth...
+def SystemState.takeNthStep (state : @SystemState ArchReqType) (acceptRequests : @ProgramState ArchReqType)
+(n : Nat) : Except String (@Transition ArchReqType × @SystemState ArchReqType) :=
+  let transitions := state.possibleTransitions acceptRequests
+  --dbg_trace s!"possible transitions: {transitions}"
+  if transitions.isEmpty then
+    throw "No more transitions possible"
+  else
+    let opTrans := transitions.get? (n.mod transitions.length)
+    match opTrans with
+      | none => unreachable!
+      | some trans => Except.map (λ st => (trans, st)) (state.applyTransition trans)
+
+def SystemState._runWithList  : @SystemState ArchReqType →  @ProgramState ArchReqType → List Nat → Except String (@SystemState ArchReqType)
+  | state, accepts, ns => match ns with
+    | [] => throw "Empty transition number list"
+    | n::ns =>
+      let runStep := state.takeNthStep accepts n
+      match runStep with
+        | Except.error "No more transitions possible" => Except.ok state
+        | Except.ok (trans,state') =>
+          -- dbg_trace trans.toString
+          -- dbg_trace state'
+          state'._runWithList (ProgramState.removeTransition accepts trans) ns
+        | Except.error e => Except.error e
+
+def SystemState.runWithList  : @SystemState ArchReqType →  @ProgramState ArchReqType → List Nat → Except String (@SystemState ArchReqType)
+  | state, accepts, ns => if !(List.join (accepts.map Array.toList).toList |>.all Transition.isAccept)
+  then throw "Running with non-accept transition inputs"
+  else SystemState._runWithList state accepts ns
+
+
+/-
+private def appendTransitionStateAux : List (List Transition × SystemState) → Transition × SystemState  → List (List Transition × SystemState)
+  | partialTrace, (trans,state) => partialTrace.map λ (transitions, _) => (trans::transitions, state)
+
+Stack overflow :
+
+-- is this DFS or BFS?
+partial def SystemState.runDFSAux (state : SystemState) (accepts : List Transition) (condition : SystemState → Bool)
+  (partialTrace : List (List Transition × SystemState)) (transition : Transition): List (List Transition × SystemState) :=
+  --dbg_trace s!"partialTrace {partialTrace.map fun (t,_) => t}"
+  --dbg_trace s!"executing {transition}"
+  let accepts' := accepts.removeAll [transition]
+  let stepExcept := state.applyTransition transition
+  match stepExcept with
+    | Except.error _ => []
+    | Except.ok state' =>
+      let partialTrace' := appendTransitionStateAux partialTrace (transition,state')
+      if condition state'
+      then partialTrace'
+      else if state'.isDeadlocked accepts'
+      then []
+      else
+        let transitions' := state'.possibleTransitions accepts'
+        List.join $ transitions'.map (state'.runDFSAux accepts' condition partialTrace')
+
+def SystemState.runDFS : SystemState → List Transition × List Transition → (SystemState → Bool) →
+  List (List Transition × SystemState)
+  | state, (inittransitions, accepts), condition =>
+  let stateinit := state.applyTrace inittransitions
+  match stateinit with
+    | .ok st =>
+      let transitions := st.possibleTransitions accepts
+      List.join $ transitions.map (st.runDFSAux accepts condition [([],state)])
+    | .error _ =>
+      --dbg_trace s!"error: {e}"
+      [(inittransitions,state)]
+-/
+-- the unapologetically imperative version:
+def SystemState.runBFS (state : @SystemState ArchReqType) (inittuple : List (@Transition ArchReqType) × @ProgramState ArchReqType)
+ (condition : @SystemState ArchReqType → Bool) (stopAtCondition : optParam Bool false) (storePartialTraces : optParam Bool false):
+ List (List (@Transition ArchReqType) × @SystemState ArchReqType) :=
+match inittuple with
+  | (inittransitions, accepts) =>
+  let stateinit := state.applyTrace inittransitions
+  match stateinit with
+    | .ok startState =>
+    Id.run do
+      -- either save the state (memory cost) or recompute it (computational cost)
+      -- we choose the former so that we can also filter out states that we've seen before
+      let mut unexplored := #[([],accepts,startState)t]
+      let mut found := []
+      dbg_trace s!"starting state {startState}"
+      dbg_trace s!"litmus requests {accepts}"
+      while  h : unexplored.size > 0 do
+          --dbg_trace s!"{unexplored.size} unexplored"
+          --dbg_trace s!"{unexplored} unexplored"
+          let unexplored_cur := unexplored[unexplored.size - 1]'(by apply n_minus_one_le_n h)
+          let partialTrace := unexplored_cur.1
+          let acceptsRemaining := unexplored_cur.2
+          let st := unexplored_cur.3
+          let transitions := st.possibleTransitions acceptsRemaining
+          --acceptsRemaining := acceptsRemaining.map $ List.removeAll [transition]
+          unexplored := unexplored.pop
+          -- if unexplored.any (λ (_,a,s) => a == acceptsRemaining && s == st') then
+          --   dbg_trace s!"this should not happen! {unexplored} contains {(partialTrace,acceptsRemaining)}"
+          --dbg_trace s!"unexplored.pop {unexplored.size}"
+          found := if condition st then (partialTrace,st)::found else found
+          unexplored := if stopAtCondition && condition st
+          then Array.mk []
+          else
+            let newPTs := transitions.map (if storePartialTraces
+                                           then λ t => t::partialTrace
+                                           else λ _ => [])
+            -- TODO: this could yield a bug if we have two identical requests in a litmus test
+            let newACs := transitions.map λ t => ProgramState.removeTransition acceptsRemaining t
+            -- let _ := transitions.any λ t => if st.canApplyTransition t
+            --   then dbg_trace s!"applied invalid transition {t} at {st}"
+            --   true
+            --   else false
+            let newSTs := transitions.map λ t => st.applyTransition! t
+            let newPairs := newACs.zip newSTs |>.filter λ pair => !unexplored.any λ (_,progState,sysState)t => pair == (progState, sysState)
+            -- why do I need to make this coe explicit?
+            let newTriples : List (Triple (List Transition) ProgramState SystemState) := newPTs.zip newPairs |>.map Coe.coe
+            unexplored.append newTriples.toArray
+            --if unexplored.size > 11337 then
+            -- dbg_trace s!"state: {st}"
+            -- dbg_trace s!"possible transitions: {transitions}"
+            --unexplored := #[]
+
+      return found
+    | .error _ =>
+    --dbg_trace s!"error: {e}"
+    [(inittransitions,state)]
+
+
+def SystemState.runBFSNoDeadlock : @SystemState ArchReqType → List (@Transition ArchReqType) × @ProgramState ArchReqType →
+List (List (@Transition ArchReqType) × @SystemState ArchReqType)
+  | state, litmus => state.runBFS litmus λ _ => false
+
+-- Doesn't work. Need to combine removed with requests
+-- def SystemState.satisfiedRequestPairs : SystemState → List (Request × Request)
+--   | state =>
+--     let pairsOpt := state.satisfied.map λ (rdId, wrId) => (state.requests.val[rdId], state.requests.val[wrId])
+--     let optPairs := pairsOpt.map λ (opRd, opWr) => match (opRd,opWr) with
+--       | (some rd, some wr) => some (rd,wr)
+--       | _ => none
+--     filterNones optPairs
+
+def SystemState.outcome : @SystemState ArchReqType → List (ThreadId × Address × Value)
+  | state =>
+    -- TODO: this won't work for reads that stay there
+    let triple := state.removed.map λ rd => (rd.thread, rd.address?.get!, rd.value?)
+    triple.toArray.qsort (λ (th,ad,_) (th',ad',_) => lexble (th,ad) (th',ad')) |>.toList
+
+-- | state, accepts => state.runDFS accepts λ _ => false
+
+    -- let runStep := λ (acceptsRemaining, state) n => state.takeNthStep acceptsRemaining n
+    -- ns.foldlM (init := (accepts, state)) runStep
+    -- ns.foldlM  (init := state) λ state.takeNthStep accepts.zip ns
