Pop/Program.lean
@@ -3,38 +3,53 @@ import Lean
 import Pop.Pop
 import Pop.Util
 import Std.Data
+import Pop.Exploration
 open Std.HashMap
 open Util
 
 namespace Pop
 
+inductive DefaultReqType
+  | mk : DefaultReqType
+  deriving BEq, Inhabited
+
+def mkRead (addr : Address) : @BasicRequest DefaultReqType :=
+  let rr : ReadRequest := { addr := addr, reads_from := none, val := none}
+  BasicRequest.read rr default
+
+def mkWrite (addr : Address) (val : Value) : @BasicRequest DefaultReqType :=
+  let wr : WriteRequest := { addr := addr, val := val}
+  BasicRequest.write wr default
+
+def mkBarrier : @BasicRequest DefaultReqType := BasicRequest.barrier default
+
 -- TODO: Add values to writes
-def mkRequest : String × Address × Value → ThreadId → Option Transition
+def mkRequest : String × Address × Value → ThreadId → Option (@Transition DefaultReqType)
   | ("R", addr, _), thId  => some $ Pop.Transition.acceptRequest (Pop.mkRead addr) thId
   | ("W", addr, val), thId  => some $ Pop.Transition.acceptRequest (Pop.mkWrite addr val) thId
   | ("Fence", _, _), thId => some $ Pop.Transition.acceptRequest (Pop.mkBarrier) thId
   | _, _ => none
 
-def initZeroesUnpropagatedTransitions : List Address → List Transition
+def initZeroesUnpropagatedTransitions : List Address → List (@Transition DefaultReqType)
   | addresses =>
   -- Does the threadId matter? For now, using 0
   addresses.map λ addr => Pop.Transition.acceptRequest (Pop.mkWrite addr 0) 0
 
-def SystemState.initZeroesUnpropagated! : SystemState → List Address → SystemState
+def SystemState.initZeroesUnpropagated! : @SystemState DefaultReqType → List Address → @SystemState DefaultReqType
   | state, addresses =>
     let writeReqs := initZeroesUnpropagatedTransitions addresses
     state.applyTrace! writeReqs
 
-def SystemState.initZeroesUnpropagated : SystemState → List Address → Except String SystemState
+def SystemState.initZeroesUnpropagated : @SystemState DefaultReqType → List Address → Except String (@SystemState DefaultReqType)
   | state, addresses =>
   let writeReqs := initZeroesUnpropagatedTransitions addresses
   state.applyTrace writeReqs
 
-def mkPropagateTransitions : List RequestId → List ThreadId → List Transition
+def mkPropagateTransitions : List RequestId → List ThreadId → List (@Transition DefaultReqType)
 | writeReqIds, threads =>
   List.join $ writeReqIds.map λ wr => threads.foldl (λ reqs thId => (Pop.Transition.propagateToThread wr thId) :: reqs) []
 
-def SystemState.initZeroesPropagateTransitions : SystemState → List Address → List Transition
+def SystemState.initZeroesPropagateTransitions : @SystemState DefaultReqType → List Address → List (@Transition DefaultReqType)
   | state, addresses =>
   let reqs := filterNones $ state.requests.val.toList
   -- this filter should be uneccessary if SystemState is empty
@@ -43,41 +58,23 @@ def SystemState.initZeroesPropagateTransitions : SystemState → List Address �
   let threads := state.system.threads.removeAll [0]
   mkPropagateTransitions writeReqIds threads
 
-def SystemState.initZeroesPropagate! : SystemState → List Address → SystemState
+def SystemState.initZeroesPropagate! : @SystemState DefaultReqType → List Address → @SystemState DefaultReqType
   | state, addresses => state.applyTrace! $ state.initZeroesPropagateTransitions addresses
-def SystemState.initZeroesPropagate : SystemState → List Address → Except String SystemState
+def SystemState.initZeroesPropagate : @SystemState DefaultReqType → List Address → Except String (@SystemState DefaultReqType)
   | state, addresses => state.applyTrace $ state.initZeroesPropagateTransitions addresses
 
-def SystemState.initZeroes! : SystemState → List Address → SystemState
+def SystemState.initZeroes! : @SystemState DefaultReqType → List Address → @SystemState DefaultReqType
   | state, addresses =>
     let unpropagated := state.initZeroesUnpropagated! addresses
     unpropagated.initZeroesPropagate! addresses
 
-def SystemState.initZeroes : SystemState → List Address → Except String SystemState
+def SystemState.initZeroes : @SystemState DefaultReqType → List Address → Except String (@SystemState DefaultReqType)
   | state, addresses =>
     let unpropagated := state.initZeroesUnpropagated addresses
     Except.bind  unpropagated (λ st => st.initZeroesPropagate addresses)
 
-abbrev ProgramState := Array (Array Transition)
-
-def ProgramState.getAvailable (prog : ProgramState) : List Transition := Id.run do
-  let mut res := []
-  for thread in prog do
-    if h : thread.size > 0 then
-    res := thread[thread.size - 1]'(by apply n_minus_one_le_n h) :: res
-  return res
-
-def ProgramState.removeTransition (prog : ProgramState) (transition : Transition)
-  : ProgramState := Id.run do
-  let mut res := #[]
-  let mut thread' := #[]
-  for thread in prog do
-    thread' := thread.erase transition
-    res := res.push thread'
-  return res
-
 -- create accepts in a per-thread basis
-def createAcceptList : List (List (String × String × Nat)) → List Transition × ProgramState
+def createAcceptList : List (List (String × String × Nat)) → List (@Transition DefaultReqType) × Array (Array (@Transition DefaultReqType))
   | list =>
   let variablesRaw := list.map λ thread => thread.map (λ r => if r.2.1.length == 0 then none else some r.2.1)
   let variables := removeDuplicates $ filterNones $ List.join variablesRaw
@@ -122,197 +119,3 @@ macro_rules
   | `(request_set| $r:request_seq || $rs:request_set) => `($r :: $rs)
 macro_rules
   | `(<| $r |>) => `( createAcceptList $r)
-
-def Request.possiblePropagateTransitions (req : Request) (state :  SystemState) : List Transition :=
-  let threads := state.system.threads.removeAll req.propagated_to
-  --dbg_trace s!"Req {req.id} has not propagated to {threads}"
-  let threads_valid := threads.filter (state.canPropagate req.id)
-  --dbg_trace s!"Req {req.id} can propagate to {threads_valid}"
-  threads_valid.map λ th => Transition.propagateToThread req.id th
-
-def SystemState.possiblePropagateTransitions (state :  SystemState) : List Transition :=
-  let requests := filterNones state.requests.val.toList
-  let requests_not_fully_propagated := requests.filter λ r => ! (@Request.fullyPropagated state.system.scopes r state.system.scopes.systemScope)
-  let removedIds := state.removed.map Request.id
-  let requests_active := requests_not_fully_propagated.filter λ r => (state.seen.elem r.id) && (!removedIds.elem r.id)
-  -- dbg_trace s!"active requests: {requests_active}"
-  List.join $ requests_active.map λ r => r.possiblePropagateTransitions state
-
-def Request.possibleSatisfyTransitions (read : Request) (state : SystemState) : List Transition :=
-  if !read.isRead then [] else
-    let requests := filterNones state.requests.val.toList
-    let writes_propagated_eq := requests.filter λ write => write.isWrite && write.propagated_to == read.propagated_to
-    --dbg_trace s!"writes with eq propagation to {read.id}: {writes_propagated_eq}"
-    let write_ids := writes_propagated_eq.map Request.id
-    let writes_valid := write_ids.filter (λ write => state.canSatisfyRead read.id write) -- should be length 1
-    --dbg_trace s!"valid writes for transition: {writes_valid}" 
-    writes_valid.map $ Transition.satisfyRead read.id
-
-def SystemState.possibleSatisfyTransitions (state :  SystemState) : List Transition :=
-  let requests := filterNones state.requests.val.toList
-  let unsatisfied_reads := requests.filter λ r => r.isRead && !(state.isSatisfied r.id)
-  List.join $ unsatisfied_reads.map λ r => r.possibleSatisfyTransitions state
-
-def SystemState.possibleTransitions (state : SystemState) (unaccepted : ProgramState) :=
-  let allaccepts := unaccepted.map λ th => th.filter Transition.isAccept
-  let accepts := ProgramState.getAvailable allaccepts
-  accepts ++ state.possibleSatisfyTransitions ++ state.possiblePropagateTransitions
-
-def SystemState.hasUnsatisfiedReads (state : SystemState) :=
-  let requests := filterNones state.requests.val.toList
-  let reads := requests.filter Request.isRead
-  let readids := reads.map Request.id
-  let unsatisfied := readids.filter state.isSatisfied
-  unsatisfied != []
-
-def SystemState.isDeadlocked (state : SystemState) (unaccepted : ProgramState) :=
-  let transitions := state.possibleTransitions unaccepted
-  transitions == [] && state.hasUnsatisfiedReads
-
--- This should be a monad transformer or smth...
-def SystemState.takeNthStep (state : SystemState) (acceptRequests : ProgramState) (n : Nat) : Except String (Transition × SystemState) :=
-  let transitions := state.possibleTransitions acceptRequests
-  --dbg_trace s!"possible transitions: {transitions}"
-  if transitions.isEmpty then
-    throw "No more transitions possible"
-  else
-    let opTrans := transitions.get? (n.mod transitions.length)
-    match opTrans with
-      | none => unreachable!
-      | some trans => Except.map (λ st => (trans, st)) (state.applyTransition trans)
-
-def SystemState._runWithList  : SystemState →  ProgramState → List Nat → Except String SystemState
-  | state, accepts, ns => match ns with
-    | [] => throw "Empty transition number list"
-    | n::ns =>
-      let runStep := state.takeNthStep accepts n
-      match runStep with
-        | Except.error "No more transitions possible" => Except.ok state
-        | Except.ok (trans,state') =>
-          -- dbg_trace trans.toString
-          -- dbg_trace state'
-          state'._runWithList (ProgramState.removeTransition accepts trans) ns
-        | Except.error e => Except.error e
-
-def SystemState.runWithList  : SystemState →  ProgramState → List Nat → Except String SystemState
-  | state, accepts, ns => if !(List.join (accepts.map Array.toList).toList |>.all Transition.isAccept)
-  then throw "Running with non-accept transition inputs"
-  else SystemState._runWithList state accepts ns
-
-
-/-
-private def appendTransitionStateAux : List (List Transition × SystemState) → Transition × SystemState  → List (List Transition × SystemState)
-  | partialTrace, (trans,state) => partialTrace.map λ (transitions, _) => (trans::transitions, state)
-
-Stack overflow :
-
--- is this DFS or BFS?
-partial def SystemState.runDFSAux (state : SystemState) (accepts : List Transition) (condition : SystemState → Bool)
-  (partialTrace : List (List Transition × SystemState)) (transition : Transition): List (List Transition × SystemState) :=
-  --dbg_trace s!"partialTrace {partialTrace.map fun (t,_) => t}"
-  --dbg_trace s!"executing {transition}"
-  let accepts' := accepts.removeAll [transition]
-  let stepExcept := state.applyTransition transition
-  match stepExcept with
-    | Except.error _ => []
-    | Except.ok state' =>
-      let partialTrace' := appendTransitionStateAux partialTrace (transition,state')
-      if condition state'
-      then partialTrace'
-      else if state'.isDeadlocked accepts'
-      then []
-      else
-        let transitions' := state'.possibleTransitions accepts'
-        List.join $ transitions'.map (state'.runDFSAux accepts' condition partialTrace')
-
-def SystemState.runDFS : SystemState → List Transition × List Transition → (SystemState → Bool) →
-  List (List Transition × SystemState)
-  | state, (inittransitions, accepts), condition =>
-  let stateinit := state.applyTrace inittransitions
-  match stateinit with
-    | .ok st =>
-      let transitions := st.possibleTransitions accepts
-      List.join $ transitions.map (st.runDFSAux accepts condition [([],state)])
-    | .error _ =>
-      --dbg_trace s!"error: {e}"
-      [(inittransitions,state)]
--/
--- the unapologetically imperative version:
-def SystemState.runBFS (state : SystemState) (inittuple : List Transition × ProgramState)
- (condition : SystemState → Bool) (stopAtCondition : optParam Bool false) : List (List Transition × SystemState) :=
-match inittuple with
-  | (inittransitions, accepts) =>
-  let stateinit := state.applyTrace inittransitions
-  match stateinit with
-    | .ok startState =>
-    Id.run do
-      let mut transitions := startState.possibleTransitions accepts
-      -- either save the state (memory cost) or recompute it (computational cost)
-      -- we choose the former so that we can also filter out states that we've seen before
-      let mut unexplored := transitions.map (λ tr => ([tr],accepts,startState))  |>.toArray
-      let mut found := []
-      let mut partialTrace := [transitions.head!]
-      let mut acceptsRemaining := #[]
-      dbg_trace s!"starting state {startState}"
-      dbg_trace s!"litmus requests {accepts}"
-      while  h : unexplored.size > 0 do
-          --dbg_trace s!"{unexplored.size} unexplored"
-          --dbg_trace s!"{unexplored} unexplored"
-          partialTrace := unexplored[unexplored.size - 1]!.1
-          acceptsRemaining := unexplored[unexplored.size - 1]!.2.1
-          let st := unexplored[unexplored.size - 1]!.2.2
-          transitions := st.possibleTransitions acceptsRemaining
-          --acceptsRemaining := acceptsRemaining.map $ List.removeAll [transition]
-          unexplored := unexplored.pop
-          -- if unexplored.any (λ (_,a,s) => a == acceptsRemaining && s == st') then
-          --   dbg_trace s!"this should not happen! {unexplored} contains {(partialTrace,acceptsRemaining)}"
-          --dbg_trace s!"unexplored.pop {unexplored.size}"
-          found := if condition st then (partialTrace,st)::found else found
-          unexplored := if stopAtCondition && condition st
-          then Array.mk []
-          else
-            let newPTs := transitions.map λ t => t::partialTrace
-            -- TODO: this could yield a bug if we have two identical requests in a litmus test
-            let newACs := transitions.map λ t => ProgramState.removeTransition acceptsRemaining t
-            let _ := transitions.any λ t => if st.canApplyTransition t
-              then dbg_trace s!"applied invalid transition {t} at {st}"
-              true
-              else false
-            let newSTs := transitions.map λ t => st.applyTransition! t
-            let newPairs := newACs.zip newSTs |>.filter λ pair => !unexplored.any λ (_,pair') => pair == pair'
-            let newTriples := newPTs.zip newPairs
-            unexplored.append newTriples.toArray
-            --if unexplored.size > 11337 then
-            -- dbg_trace s!"state: {st}"
-            -- dbg_trace s!"possible transitions: {transitions}"
-            --unexplored := #[]
-
-      return found
-    | .error _ =>
-    --dbg_trace s!"error: {e}"
-    [(inittransitions,state)]
-
-
-def SystemState.runBFSNoDeadlock : SystemState → List Transition × ProgramState → List (List Transition × SystemState)
-  | state, litmus => state.runBFS litmus λ _ => false
-
--- Doesn't work. Need to combine removed with requests
--- def SystemState.satisfiedRequestPairs : SystemState → List (Request × Request)
---   | state =>
---     let pairsOpt := state.satisfied.map λ (rdId, wrId) => (state.requests.val[rdId], state.requests.val[wrId])
---     let optPairs := pairsOpt.map λ (opRd, opWr) => match (opRd,opWr) with
---       | (some rd, some wr) => some (rd,wr)
---       | _ => none
---     filterNones optPairs
-
-def SystemState.outcome : SystemState → List (ThreadId × Address × Value)
-  | state =>
-    -- TODO: this won't work for reads that stay there
-    let triple := state.removed.map λ rd => (rd.thread, rd.address?.get!, rd.value?)
-    triple.toArray.qsort (λ (th,ad,_) (th',ad',_) => lexble (th,ad) (th',ad')) |>.toList
-
--- | state, accepts => state.runDFS accepts λ _ => false
-
-    -- let runStep := λ (acceptsRemaining, state) n => state.takeNthStep acceptsRemaining n
-    -- ns.foldlM (init := (accepts, state)) runStep
-    -- ns.foldlM  (init := state) λ state.takeNthStep accepts.zip ns
